theories/Translations/LustreAstToLustre.v
@@ -65,6 +65,7 @@ Proof.
       | Source.Bop_mult, existT _ Target.TInt e1, existT _ Target.TInt e2 => Result.Ok (existT _ _ (Target.EBinop Target.Bop_mult e1 e2))
       | Source.Bop_div, existT _ Target.TInt e1, existT _ Target.TInt e2 => Result.Ok (existT _ _ (Target.EBinop Target.Bop_div e1 e2))
       | Source.Bop_eq, existT _ Target.TInt e1, existT _ Target.TInt e2 => Result.Ok (existT _ _ (Target.EBinop Target.Bop_eq e1 e2))
+      | Source.Bop_neq, existT _ Target.TInt e1, existT _ Target.TInt e2 => Result.Ok (existT _ _ (Target.EBinop Target.Bop_neq e1 e2))
       | Source.Bop_le, existT _ Target.TInt e1, existT _ Target.TInt e2 => Result.Ok (existT _ _ (Target.EBinop Target.Bop_le e1 e2))
       | Source.Bop_lt, existT _ Target.TInt e1, existT _ Target.TInt e2 => Result.Ok (existT _ _ (Target.EBinop Target.Bop_lt e1 e2))
       | Source.Bop_ge, existT _ Target.TInt e1, existT _ Target.TInt e2 => Result.Ok (existT _ _ (Target.EBinop Target.Bop_ge e1 e2))
